finish instantiation_sound_simpl

theories/instantiation_properties.v
@@ -1,12 +1,17 @@
-From mathcomp Require Import ssreflect ssrbool ssrnat eqtype seq.
+From mathcomp Require Import ssreflect ssrbool eqtype seq.
+From mathcomp Require ssrnat.
 From ITree Require Import ITree.
 From ITree Require ITreeFacts.
-From Wasm Require Import list_extra datatypes datatypes_properties
+From stdpp Require Import list fin_maps gmap base.
+From Wasm Require Import list_extra datatypes datatypes_properties properties
                          interpreter binary_format_parser operations
                          typing opsem type_checker memory memory_list instantiation.
+Require Export stdpp_aux.
 From Coq Require Import BinNat.
 
 Section Host.
+
+Check seq.
 
 Variable host_function : eqType.
 Let host := host host_function.
@@ -33,8 +38,9 @@ Let instantiate := instantiate host_function host_instance.
 Let instantiate_simpl := instantiate_simpl host_function.
 (*
 Let tab_agree := @typing.tab_agree host_function.
-*)
-Inductive ext_typing_list: store_record -> seq module_export -> seq extern_t -> Prop :=
+ *)
+
+Inductive ext_typing_list: store_record -> seq.seq module_export -> seq.seq extern_t -> Prop :=
 | ext_typing_list_nil: forall s,
     ext_typing_list s [::] [::]
 | ext_typing_list_cons: forall s v_exp v_exps te tes,
@@ -42,64 +48,192 @@ Inductive ext_typing_list: store_record -> seq module_export -> seq extern_t -> 
     external_typing s (modexp_desc v_exp) te ->
     ext_typing_list s (v_exp :: v_exps) (te :: tes).
 
+Print alloc_funcs.
+
+Print alloc_func.
+
+Print module_func.
+
+(* This is the key definition: we should really be able to tell what the allocated new function closures are from the information of alloc_funcs. However, we need to formulate this in a way that is convenient for the other parts of the proofs. *)
+Definition alloc_funcs_new_closures (modfuncs: list module_func) (inst: instance) : list (function_closure host_function) :=
+  List.map (fun (mf: module_func) => 
+              (FC_func_native inst
+                              (List.nth match mf.(modfunc_type) with
+                                        | Mk_typeidx n => n
+                                        end
+                                        (inst.(inst_types)) (Tf [::] [::]))
+                              mf.(modfunc_locals)
+                              mf.(modfunc_body))) modfuncs.
+
+(* Same for this, but this is easier to define -- we should also be able to tell what the allocated function indices are. *)
+
 (*
-Lemma instantiation_sound (s: store_record) m v_imps s' inst v_exps start:
-  store_typing s ->
-  instantiate s m v_imps ((s', inst, v_exps), start) ->
-  (store_typing s') /\
-  (exists C, inst_typing s' inst C) /\
-  (exists tes, ext_typing_list s' v_exps tes) /\
-  (pred_option (fun i => i < length s'.(s_funcs)) start).
-  (* /\ store_extension s s' *)
+Fixpoint nat_list (acc: list nat) (n : nat) : list nat :=
+  match n with
+  | O => acc
+  | (S n') => nat_list (n' :: acc) n'
+  end.
+ 
+Lemma nat_list_length: forall acc n,
+  length (nat_list acc n) = length acc + n.
 Proof.
 Admitted.
 
-Let tab_agree := @tab_agree host_function.
+Lemma 
 
-Lemma tab_agree_aux s_funcs s_tables s_mems s_globals tab func:
-  tab_agree {| s_funcs := s_funcs; s_tables := s_tables; s_mems := s_mems; s_globals := s_globals |} tab ->
-  tab_agree {| s_funcs := List.app s_funcs [:: func]; s_tables := s_tables; s_mems := s_mems;
-               s_globals := s_globals |} tab .
+i < n -> 
+List.nth_error (nat_list acc n) i = Some i.
+
+Lemma 
+i >= n -> 
+List.nth_error (nat_list acc n) i = List.nth_error acc (i - n).
+*)
+
+Definition gen_index offset len : list nat :=
+  imap (fun i x => i+offset+x) (repeat 0 len).
+
+Lemma gen_index_len offset len:
+  length (gen_index offset len) = len.
 Proof.
-  rewrite /tab_agree /typing.tab_agree.
-  move => Htb.
-  destruct Htb as [Htable Hs_tables]; subst.
-  constructor.
-  - (* forall tabcl_agree (table_data tab) *)
-    induction (table_data tab) as [| hd tl IH]; first by constructor.
-    (* forall tabcl_agree hd :: tl *)
-    inversion Htable as [| x y Hhd Htl]; subst.
-    constructor.
-    (* tabcl_agree hd *)
-    destruct hd => //=. 
-    rewrite /tabcl_agree in Hhd. simpl in Hhd.
-    rewrite size_cat. by rewrite ltn_addr.
-    (* forall tabcl_agree tl *)
-    apply IH. exact Htl.
-  - (* tabsize_agree table *)
-    assumption.
+  unfold gen_index.
+  rewrite imap_length.
+  by rewrite repeat_length.
+Qed.
+  
+Lemma gen_index_lookup offset len k:
+  k < len ->
+  (gen_index offset len) !! k = Some (offset + k).
+Proof.
+  move => Hlen.
+  unfold gen_index.
+  rewrite list_lookup_imap => /=.
+  eapply repeat_lookup with (x := 0) in Hlen.
+  rewrite Hlen.
+  simpl.
+  f_equal.
+  by lias.
 Qed.
 
-Let functions_agree := @functions_agree host_function.
-
-Lemma functions_agree_aux s_funcs func f tf: 
-  functions_agree s_funcs f tf ->
-  functions_agree (List.app s_funcs [:: func]) f tf.
+Lemma gen_index_extend offset len:
+  gen_index offset (len+1) = gen_index offset len ++ [::offset+len].
 Proof.
-  rewrite /functions_agree /typing.functions_agree.
-  move/andP => [H1 H2]. move/eqP in H2.
-  apply/andP. split.
-  + (* f < length (s_funcs [::func])  *)
-    rewrite List.app_length.
-    by rewrite ltn_addr.
-  + (* option_map cl_type (List.nth_error (s_funcs [::func]) f) == Some tf *)
-    apply/eqP.
-    rewrite <-H2.
-    apply f_equal.
-    apply List.nth_error_app1.
-    by apply/ltP.
+  unfold gen_index.
+  rewrite repeat_app => /=.
+  induction len => //=.
+  f_equal => //.
+  do 2 rewrite - fmap_imap.
+  rewrite IHlen.
+  rewrite fmap_app => /=.
+  repeat f_equal.
+  by lias.
 Qed.
 
+Lemma gen_index_in x offset len:
+  In x (gen_index offset len) ->
+  x < offset + len.
+Proof.
+Admitted.
+
+(*
+Definition alloc_funcs_new_indices (ws: store_record) (modfuncs: list module_func) : list funcidx :=
+  List.map (fun n => Mk_funcidx (n + List.length ws.(s_funcs))) (nat_list nil (List.length modfuncs)).
+ *)
+
+(*
+Definition alloc_funcs_new_indices (ws : store_record) (modfuncs: list module_func) : list funcidx :=
+  List.map Mk_funcidx (gen_index (length (s_funcs ws)) (length modfuncs)).
+
+Lemma alloc_func_ws_res modfuncs ws inst ws' l:
+  (ws', l) = alloc_funcs host_function ws modfuncs inst ->
+  ws'.(s_funcs) = ws.(s_funcs) ++ alloc_funcs_new_closures modfuncs inst /\
+  ws'.(s_tables) = ws.(s_tables) /\
+  ws'.(s_mems) = ws.(s_mems) /\
+  ws'.(s_globals) = ws.(s_globals).
+Proof.
+  move: l ws' ws. Check List.rev_ind.
+  induction modfuncs using List.rev_ind; move => l ws' ws Halloc => /=.
+
+  (* modfuncs = nil *)
+  - inversion Halloc; subst.
+    split => //=; first by rewrite -> List.app_nil_r.
+
+  (* modfuncs = modfuncs ++ [:: x] *)
+  - rewrite /alloc_funcs /alloc_Xs in Halloc.
+    
+    rewrite List.fold_left_app in Halloc.
+    remember (List.fold_left _ modfuncs (ws, [::])) as temp_ws_l.
+    destruct temp_ws_l as [ws_i l_i].
+    
+    simpl in Halloc.
+    specialize (IHmodfuncs (List.rev l_i) ws_i ws). 
+    destruct IHmodfuncs as [Hfunc [Htab [Hmem Hglob]]].
+    {
+      rewrite /alloc_funcs /alloc_Xs.
+      by rewrite <- Heqtemp_ws_l.
+    }
+    {
+      rewrite /add_func in Halloc.
+      inversion Halloc. simpl.
+      split.     
+      + (* s_funcs ws_i ++ x_func_inst = s_funcs ws ++ alloc_funcs_new (modfuncs ++ [:: x]) *)
+        rewrite /alloc_funcs_new_closures.
+        rewrite List.map_app. simpl.
+        rewrite -> List.app_assoc.
+        f_equal. exact Hfunc.
+      + (* s_tables /\ s_mems /\ s_globals *)
+        by split => //=.
+    }
+Qed.
+ *)
+
+Definition gen_func_instance mf inst : function_closure host_function :=
+  let ft := nth match modfunc_type mf with
+                | Mk_typeidx n => n
+                end (inst_types inst) (Tf [] []) in
+  FC_func_native inst ft (modfunc_locals mf) (modfunc_body mf).
+
+Lemma alloc_func_gen_index (modfuncs : list module_func)  ws inst ws' l:
+  alloc_funcs host_function ws modfuncs inst = (ws', l) ->
+  map (fun x => match x with | Mk_funcidx i => i end) l = gen_index (length (s_funcs ws)) (length modfuncs) /\
+  ws'.(s_funcs) = ws.(s_funcs) ++ fmap (fun mf => gen_func_instance mf inst) modfuncs /\
+ (* length ws'.(s_funcs) = length ws.(s_funcs) + length modfuncs /\*)
+  ws.(s_tables) = ws'.(s_tables) /\
+  ws.(s_mems) = ws'.(s_mems) /\
+  ws.(s_globals) = ws'.(s_globals).
+Proof.
+  unfold alloc_funcs, alloc_Xs.
+  generalize dependent l.
+  generalize dependent ws'.
+  generalize dependent ws.
+  induction modfuncs using List.rev_ind; move => ws ws' l Hallocfuncs.
+  -
+    inversion Hallocfuncs; subst; clear Hallocfuncs.
+    simpl.
+    repeat split => //.
+    by rewrite app_nil_r.
+  - rewrite fold_left_app in Hallocfuncs.
+    remember (fold_left _ modfuncs (ws,[])) as fold_res.
+    simpl in Hallocfuncs.
+    destruct fold_res as [ws0 l0].
+    symmetry in Heqfold_res. (* ? *)
+    unfold add_func in Hallocfuncs.
+
+    inversion Hallocfuncs; subst; clear Hallocfuncs.
+    rewrite map_app app_length /=. (* (rev l0 ++ [Mk_funcidx (length (s_funcs ws0))]) *)
+    rewrite gen_index_extend.
+    specialize (IHmodfuncs ws ws0 (rev l0)).
+    destruct IHmodfuncs as [? [? [? [? ?]]]]; first by rewrite Heqfold_res.
+    
+    repeat split => //; try by eapply IHmodfuncs; rewrite Heqfold_res.
+    + rewrite H.
+      rewrite H0.
+      Locate "^~".
+      by rewrite app_length map_length.
+    + rewrite H0.
+      rewrite - app_assoc.
+      f_equal.
+      by rewrite -> list_fmap_app.
+Qed.
 
 Lemma all2_forward: forall A B (f1 f2 : A -> B -> bool) l1 l2,
   (forall a b, f1 a b -> f2 a b) ->
@@ -113,17 +247,44 @@ Proof.
     + by apply E.
     + by apply IH => //=.
 Qed.
+(* 
+all2 g l1 l2 /\ all2 h l1 l2 -> 
+all2 (fun a b => (g a b) && (h a b)) l1 l2 
+
+ *)
+
+Lemma all2_and: forall A B (f g h : A -> B -> bool) l1 l2,
+    (forall a b, f a b = (g a b) && (h a b)) -> 
+    all2 g l1 l2 /\ all2 h l1 l2 -> 
+    all2 f l1 l2.
+Proof.
+Admitted.
+
+Let functions_agree := @functions_agree host_function.
+
+Lemma functions_agree_aux s_funcs funcs f tf: 
+  functions_agree s_funcs f tf ->
+  functions_agree (List.app s_funcs funcs) f tf.
+Proof.
+  rewrite /functions_agree /typing.functions_agree.
+  move/andP => [H1 H2]. move/eqP in H2.
+  apply/andP. split.
+  + (* f < length (s_funcs [::func])  *)
+    rewrite app_length.
+    by rewrite ssrnat.ltn_addr.
+  + (* option_map cl_type (List.nth_error (s_funcs [::func]) f) == Some tf *)
+    apply/eqP.
+    rewrite <-H2.
+    apply f_equal.
+    apply nth_error_app1.
+    by apply/ssrnat.ltP.
+Qed.
 
 Let cl_type_check_single := @cl_type_check_single host_function.
 
-Lemma cl_type_check_single_aux1 s_funcs s_tables s_mems s_globals inst m_f func:
+Lemma cl_type_check_single_aux s_funcs s_tables s_mems s_globals func funcs:
   cl_type_check_single {| s_funcs := s_funcs; s_tables := s_tables; s_mems := s_mems; s_globals := s_globals |} func ->
-  cl_type_check_single {| s_funcs := s_funcs ++ 
-                                     [:: FC_func_native inst
-                                         (List.nth match modfunc_type m_f with
-                                            | Mk_typeidx n => n
-                                            end (inst_types inst) (Tf [::] [::])) (modfunc_locals m_f) 
-                                         (modfunc_body m_f)]; 
+  cl_type_check_single {| s_funcs := s_funcs ++ funcs; 
                           s_tables := s_tables; s_mems := s_mems; s_globals := s_globals |} func.
 Proof.
   move => Hcl.
@@ -161,198 +322,268 @@ Proof.
     by apply cl_typing_host.
 Qed.
 
-Lemma store_typing_preserve_add_func : forall s_funcs s_tables s_mems s_globals inst m_f,
-    store_typing
-      {| s_funcs := s_funcs; s_tables := s_tables; s_mems := s_mems; s_globals := s_globals |} ->
-    (*
-    add_func s _ _ ...
-*)
-    store_typing
-      {| s_funcs :=
-        List.app s_funcs
-                 [:: FC_func_native
-                     inst
-                     (List.nth (match m_f.(modfunc_type) with | Mk_typeidx n => n end) inst.(inst_types) (Tf nil nil))
-                     m_f.(modfunc_locals)
-                     m_f.(modfunc_body)]
-      ; s_tables := s_tables; s_mems := s_mems; s_globals := s_globals |}.
-Proof.
-  move=> s_funcs s_tables s_mems s_globals inst m_f HSTyping.
-  Print store_typing.
-  inversion HSTyping as [Hcl [ Htb Hmem ]].
-  constructor.
-  - (* cl_typing *)
-    rewrite List.Forall_app.
-    split.
-    + (* forall cl_type_check_single s_funcs *) 
-      apply List.Forall_forall => func Hin.
-      rewrite -> List.Forall_forall in Hcl.
-      apply cl_type_check_single_aux1.
-      by apply Hcl.
-    + (* cl_typing_check_single func *) {
-        constructor => //=.
-        remember (List.nth match modfunc_type m_f with
-                           | Mk_typeidx n => n
-                           end (inst_types inst) (Tf [::] [::])) as tf.
-        exists tf.
-        destruct tf as [t1s t2s]. Check List.map.  Search (N).
-        remember ({| tc_types_t := inst.(inst_types);
-                     tc_func_t := (List.map cl_type s_funcs) ++ [:: (Tf t1s t2s)];
-                     tc_global := List.map (fun g => Build_global_type (g_mut g) (typeof (g_val g))) s_globals;
-                     tc_table := List.map
-                                 (fun t => {| tt_limits := {| lim_min := N.of_nat(tab_size t);
-                                                              lim_max := Some (N.of_nat(t.(table_max_opt) + 1)) |};
-                                              tt_elem_type := ELT_funcref |})
-                                 s_tables;
-                     tc_memory := List.map
-                                  (fun m => {| lim_min := (mem_size m); lim_max := m.(mem_max_opt) |})
-                                s_mems;
-                     tc_local := nil;
-                     tc_label := nil;
-                    tc_return := None |}) as C.
-        apply cl_typing_native with
-          (C := C)
-          (C' := upd_local_label_return C (tc_local C ++ t1s ++ (modfunc_locals m_f)) ([::t2s] ++ tc_label C) (Some t2s)) => //=.
-        * (* inst_typing *)
-          admit. admit.
-          (*
-          destruct inst. destruct C. simpl.
-          destruct tc_local => //=.
-          destruct tc_label => //=.
-          destruct tc_return => //=.
-          inversion HeqC; subst.
-          destruct HeqC. 
-          apply/andP. split.
-          apply/andP. split.
-          apply/andP. split.
-          apply/andP. split => //=.
-          -- (* functions_agree *) {
-            admit.
-          }
-          -- (* globals_agree *) {
-              rewrite /globals_agree.
-              admit.
-            }
-*)
-      }
-  split.
-  - (* tab_agree *)
-    apply List.Forall_forall => tab Hin.
-    rewrite -> List.Forall_forall in Htb.
-    apply tab_agree_aux.
-    by apply Htb.
-  - (* mem_agree *)
-    assumption.
-Admitted.
+Let tab_agree := @tab_agree host_function.
 
-Lemma instantiation_sound_aux s s0 mfuncs inst l acc:
-  store_typing s ->
-  (s0, l) =
-           (let
-            '(s', fas) :=
-             List.fold_left
-               (fun '(s, ys) (x : module_func)
-                  => let '(s', y) := alloc_func host_function s x inst in (s', y :: ys))
-               mfuncs (s, acc) in (s', List.rev fas)) ->
-  store_typing s0.
+Lemma tab_agree_aux s_funcs s_tables s_mems s_globals tab funcs:
+  tab_agree {| s_funcs := s_funcs; s_tables := s_tables; s_mems := s_mems; s_globals := s_globals |} tab ->
+  tab_agree {| s_funcs := s_funcs ++ funcs; s_tables := s_tables; s_mems := s_mems;
+               s_globals := s_globals |} tab .
 Proof.
-  generalize dependent s.
-  generalize dependent acc.
-  induction mfuncs => //; move => acc s HType H0.
-  - simpl in H0.
-    by inversion H0; subst.
-  - simpl in H0.
-    apply IHmfuncs in H0 => //.
-    unfold add_func. 
-    apply store_typing_preserve_add_func.
-    by destruct s => //.
+  rewrite /tab_agree /typing.tab_agree.
+  move => Htb.
+  destruct Htb as [Htable Hs_tables]; subst.
+  constructor.
+  - (* forall tabcl_agree (table_data tab) *)
+    induction (table_data tab) as [| hd tl IH]; first by constructor.
+    (* forall tabcl_agree hd :: tl *)
+    inversion Htable as [| x y Hhd Htl]; subst.
+    constructor.
+    (* tabcl_agree hd *)
+    destruct hd => //=. 
+    rewrite /tabcl_agree in Hhd. simpl in Hhd.
+    rewrite size_cat. by rewrite ssrnat.ltn_addr.
+    (* forall tabcl_agree tl *)
+    apply IH. exact Htl.
+  - (* tabsize_agree table *)
+    assumption.
 Qed.
-*)
 
 (*
-Lemma instantiation_sound_simpl:  forall (s: store_record) m v_imps s' inst v_exps start,
-  store_typing s ->
-  instantiate_simpl s m v_imps ((s', inst, v_exps), start) ->
-  (store_typing s').
-  (* (exists C, inst_typing s' inst C) /\
-  (exists tes, ext_typing_list s' v_exps tes) /\
-  (pred_option (fun i => i < length s'.(s_funcs)) start).*)
-  (* /\ store_extension s s' *)
-Proof.
-  move=> s m v_imps s' inst v_exps start HType HInst. inversion HInst.
-  remember (alloc_funcs host_function s (mod_funcs m) inst) as psi.
-  destruct psi.
-  rewrite /alloc_funcs /alloc_Xs in Heqpsi.
-  apply instantiation_sound_aux in Heqpsi => //.
-  simpl in Heqpsi.
-  move/andP in Heqpsi.
-  destruct H0 as [Heqs Heqinst].
-  move/eqP in Heqs; subst.
-  move/eqP in Heqinst.
-  apply instantiation_sound_aux in Heqpsi => //.
-Qed.*)
-
-
-Print alloc_funcs.
-
-Print alloc_func.
-
-Print module_func.
-
-(* This is the key definition: we should really be able to tell what the allocated new function closures are from the information of alloc_funcs. However, we need to formulate this in a way that is convenient for the other parts of the proofs. *)
-Definition alloc_funcs_new_closures (modfuncs: list module_func) (inst: instance) : list (function_closure host_function) :=
-  List.map (fun (mf: module_func) => 
-              (FC_func_native inst
-                              (List.nth match mf.(modfunc_type) with
-                                        | Mk_typeidx n => n
-                                        end
-                                        (inst.(inst_types)) (Tf [::] [::]))
-                              mf.(modfunc_locals)
-                              mf.(modfunc_body))) modfuncs.
-
-(* Same for this, but this is easier to define -- we should also be able to tell what the allocated function indices are. *)
-Definition alloc_funcs_new_indices (ws: store_record) (modfuncs: list module_func) : list funcidx.
-Admitted.
-
-Lemma alloc_func_ws_res modfuncs ws inst ws' l:
-  (ws', l) = alloc_funcs host_function ws modfuncs inst ->
-  ws'.(s_funcs) = ws.(s_funcs) ++ alloc_funcs_new_closures modfuncs inst /\
-  ws'.(s_tables) = ws.(s_tables) /\
-  ws'.(s_mems) = ws.(s_mems) /\
-  ws'.(s_globals) = ws.(s_globals).
-Proof.
-  move: l ws' ws.
-  induction modfuncs using List.rev_ind; move => l ws' ws Halloc => /=.
-Admitted.
-    
-Lemma alloc_func_index_res modfuncs ws inst ws' l:
-  (ws', l) = alloc_funcs host_function ws modfuncs inst ->
-  l = alloc_funcs_new_indices ws modfuncs.
+Lemma forall2_length: forall A B R (l1 : seq.seq A) (l2 : seq.seq B),
+    List.Forall2 R l1 l2 -> List.length l1 = List.length l2.
 Proof.
 Admitted.
-  
+ *)
+
+
+
+Lemma nth_error_lookup {T: Type} (l: list T) i:
+  nth_error l i = l !! i.
+Proof.
+  move: i.
+  by induction l; move => i; destruct i => //=.
+Qed.
+
+
+(* similar to Forall2_lookup_lr 
+Forall2_lookup_lr:
+  ∀ (A B : Type) (P : A → B → Prop) (l : seq.seq A) (k : seq.seq B) (i : nat) (x : A) (y : B),
+    Forall2 P l k → l !! i = Some x → k !! i = Some y → P x y
+*)
+Lemma Forall2_nth_error: forall A B R (l1 : seq.seq A) (l2 : seq.seq B) n m k,
+    List.Forall2 R l1 l2 ->
+    List.nth_error l1 n = Some m ->
+    List.nth_error l2 n = Some k ->
+    R m k.
+Proof.
+Admitted.
+
+
+Search Forall2.
+(* similar to Forall2_same_length_lookup_2
+Forall2_same_length_lookup_2:
+  ∀ (A B : Type) (P : A → B → Prop) (l : seq.seq A) (k : seq.seq B),
+    length l = length k
+    → (∀ (i : nat) (x : A) (y : B), l !! i = Some x → k !! i = Some y → P x y) → Forall2 P l k
+*)
+Lemma Forall2_lift: forall A B (R : A -> B -> Prop) (l1 : seq.seq A) (l2 : seq.seq B),
+    List.length l1 = List.length l2 -> 
+    (forall n m k,
+    List.nth_error l1 n = Some m -> 
+    List.nth_error l2 n = Some k ->
+    R m k) ->
+    List.Forall2 R l1 l2.
+Proof.
+Admitted.
+
+
+Lemma Forall2_all2: forall A B (R : A -> B -> bool ) (l1 : seq.seq A) (l2 : seq.seq B),
+    List.Forall2 R l1 l2 = all2 R l1 l2.
+Proof.
+Admitted.
+
+
 Lemma alloc_func_sound s s' ifs mod_funcs mod_types fts inst t_context: 
   (s', ifs) = alloc_funcs host_function s mod_funcs inst ->
   List.Forall2 (module_func_typing t_context) mod_funcs fts ->
   t_context.(tc_func_t) = fts ->
   t_context.(tc_types_t) = mod_types ->
+  t_context.(tc_global) = nil ->
+  t_context.(tc_table) = nil -> 
+  t_context.(tc_memory) = nil ->
+  t_context.(tc_local) = nil ->
+  t_context.(tc_label) = nil ->
+  t_context.(tc_return) = None ->
   inst.(inst_types) = mod_types ->
   inst.(inst_funcs) = List.map (fun '(Mk_funcidx i) => i) ifs ->
+  inst.(inst_globs) = nil ->
+  inst.(inst_tab) = nil ->
+  inst.(inst_memory) = nil -> 
   store_typing s ->
   store_typing s'.
 Proof.
   destruct inst, t_context.
-  move => Halloc Hftstype ? ? ? ? Hstoretype; simpl in *; subst.
+  move => Halloc Hftstype ? ? ? ? ? ? ? ? ? ? ? ? ? Hstoretype; simpl in *; subst.
   
   (* Doing induction on mod_funcs is hard since we only have the module validity result for the original module. 
      Instead, note that we can explicitly evaluate what the new store s' is -- intuitively, it should only differ with the original store in the function component, where a few functions are appended. *)
-  specialize (alloc_func_ws_res _ _ _ _ _ Halloc) as Hfuncres.
-  specialize (alloc_func_index_res _ _ _ _ _ Halloc) as Hindexres.
   
-  destruct Hfuncres as [Hfunc [Htab [Hmem Hglob]]].
+  specialize (alloc_func_gen_index _ _ _ _ _ (symmetry Halloc)) as Hfuncidx.
+  destruct Hfuncidx as [Hidx [Hfunc [Htab [Hmem Hglob]]]].
 
   (* We have established a relationship between the new store and the old store without using fold_left. We now have to prove the rest. Some of the lemmas proven previously commented out for now) is applicable, but need to be in a more generalised form. *)
+  
+  destruct s'. destruct s. simpl in *. destruct Hstoretype as [Hcl [Htab_agree Hmem_agree]].
+  split; rewrite -> Hfunc; subst.
+  - (* cl_type *)
+    remember ((λ mf : module_func, gen_func_instance mf _) <$> mod_funcs) as s_funcs_new.
+    rewrite -> List.Forall_app.
+    split.
+    + (* forall cl_type_check s' s_funcs0 *)
+      apply List.Forall_forall => fc Hin.
+      apply cl_type_check_single_aux.
+      rewrite -> List.Forall_forall in Hcl.
+      by apply Hcl.
+    + (* forall cl_type_check s' s_funcs_new *)
+      rewrite List.Forall_forall => fc Hin.
+      rewrite -> Heqs_funcs_new in Hin.
+      rewrite /gen_func_instance in Hin.
+      simpl in Hin.
+      eapply List.In_nth_error in Hin.
+      destruct Hin as [n Hnth].
+      rewrite Coqlib.list_map_nth in Hnth.
+      rewrite /Coqlib.option_map in Hnth.
+      destruct (nth_error mod_funcs n) eqn: Heqm => //=.
+      inversion Hnth. clear Hnth.
+      rename H0 into Heq_fc.
+      
+      assert (Hex_ty: exists ty, List.nth_error fts n = Some ty).
+      {
+        rewrite nth_error_lookup in Heqm.
+        specialize (Forall2_lookup_l _ _ _ _ _  Hftstype Heqm) as H1.
+        destruct H1 as [ty [Heqy _]].
+        rewrite <- nth_error_lookup in Heqy.
+        by exists ty.
+      }
 
+      destruct Hex_ty as [ty Hty].
+      specialize (Forall2_nth_error _ _ _ _ _ n m ty Hftstype Heqm Hty) as Hftstype_n.
+
+      rewrite /typing.cl_type_check_single.
+      destruct ty as [t1s t2s]. 
+      exists (Tf t1s t2s).
+      remember (Build_t_context mod_types fts nil nil nil nil nil None) as C.
+
+      eapply cl_typing_native with (C := C) => //=.
+
+      { (* inst_typing store inst C *)
+        destruct C.
+        destruct tc_local => //=.
+        destruct tc_label => //=.
+        destruct tc_return => //=.
+        inversion HeqC; subst.
+        destruct HeqC. 
+        apply/andP. split => //=.
+        apply/andP. split => //=.
+        apply/andP. split => //=.
+        apply/andP. split => //=.
+        { (* functions_agree *)
+          rewrite /gen_func_instance. simpl.
+          rewrite /typing.functions_agree.
+          eapply all2_and with (g := (fun n0 f => ssrnat.leq (S n0) _)) => //=.
+          split.
+          {
+            rewrite <- Forall2_all2.
+            rewrite List.app_length.
+            rewrite fmap_length.
+            rewrite Hidx.
+            apply Forall_Forall2_l.
+            (*
+              Forall_Forall2_l: ∀ (A B : Type) (P : A → B → Prop) (l : seq.seq A) (k : seq.seq B),
+                length l = length k → Forall (λ x : A, ∀ y : B, P x y) l → Forall2 P l k
+             *)
+            - rewrite gen_index_len.
+              by apply Forall2_length in Hftstype.
+            - rewrite Forall_forall.
+              move => x Hin _.
+              apply gen_index_in in Hin.
+              by move/ssrnat.ltP in Hin.
+          }
+          {
+            clear n m Heqm t1s t2s Hty Hftstype_n.
+            rewrite /module_func_typing in Hftstype; simpl in Hftstype.
+            rewrite <- Forall2_all2.
+            assert (Hlen: length ifs = length mod_funcs).
+            {
+              rewrite <- gen_index_len with (offset := (length s_funcs0)).
+              rewrite <- Hidx.
+              by rewrite map_length.
+            }
+            apply Forall2_lift.
+            - (* length (map (λ '(Mk_funcidx i), i) ifs) = length fts *)
+              rewrite map_length.
+              rewrite Hlen.
+              by apply Forall2_length in Hftstype.
+            - 
+              move => i fidx ft Hfuncs_nth Hfts_nth.
+              assert (Hnth: i < length mod_funcs).
+              {
+                rewrite Coqlib.list_map_nth in Hfuncs_nth.
+                destruct (List.nth_error ifs i) eqn:Hnth_i => //=.
+                assert (H: List.nth_error ifs i <> None) by rewrite Hnth_i => //.
+                apply List.nth_error_Some in H.
+                by rewrite <- Hlen.
+              }
+              rewrite Hidx in Hfuncs_nth.
+              rewrite nth_error_lookup in Hfuncs_nth.
+              rewrite gen_index_lookup in Hfuncs_nth => //.
+              (* todo: length l1 = length l2 -> l1 !! i = Some m -> exists, l2 !! i = Some n *)
+              apply List.nth_error_Some in Hnth.
+              destruct (List.nth_error mod_funcs i) eqn: Hmod_funcs_i => //=.
+              clear Hnth.
+              specialize (Forall2_nth_error _ _ _ _ _ _ _ _ Hftstype Hmod_funcs_i Hfts_nth) as Hftstype_n.
+              simpl in Hftstype_n.
+              simpl in Hfuncs_nth.
+              destruct m. destruct modfunc_type. destruct ft as [t1s t2s].
+              destruct Hftstype_n as [_ [Hft _]].
+              inversion Hfuncs_nth; subst.
+              clear Hfuncs_nth.
+              rewrite nth_error_app2; last by lias.
+              Search "-".
+              replace (length s_funcs0 + i - length s_funcs0) with i; last by lias.
+              Search fmap lookup.
+              rewrite nth_error_lookup.
+              rewrite list_lookup_fmap.
+              rewrite nth_error_lookup in Hmod_funcs_i.
+              rewrite Hmod_funcs_i. by simpl.
+          }
+        }
+    }
+    { (* the type index of function m references type (Tf t1s t2s) in mod_types *)
+      rewrite /module_func_typing in Hftstype_n.
+      destruct m. simpl.
+      destruct modfunc_type as [i].
+      destruct Hftstype_n as [_ [Hnth _]].
+      move/eqP in Hnth.
+      rewrite <- Hnth.
+      by inversion HeqC.
+    }
+    { (* be_typing *)
+      rewrite /module_func_typing in Hftstype_n.
+      rewrite /upd_local_label_return.
+      destruct m. simpl.
+      destruct modfunc_type.
+      destruct Hftstype_n as [_ [_ Hbe_typing]].
+      by apply Hbe_typing.
+    }
+  split.
+  - (* tab_agree *)
+    apply List.Forall_forall => tab Hin.
+    rewrite -> List.Forall_forall in Htab_agree.
+    apply tab_agree_aux.
+    by apply Htab_agree.
+  - (* mem_agree *)
+    assumption. 
 Admitted.
 
 Definition module_restriction (m: module) : Prop :=
