theories/stdpp_aux.v
@@ -1,0 +1,114 @@
+From mathcomp Require Import ssreflect eqtype seq ssrbool.
+From stdpp Require Import list fin_maps gmap.
+Require Import list_extra properties.
+
+Lemma map_fmap {T1 T2: Type} (f: T1 -> T2) (l: list T1):
+  map f l = fmap f l.
+Proof.
+  trivial.
+Qed.
+
+Lemma fmap_split: forall {X Y:Type} (f: X -> Y) vs es1 es2,
+  fmap f vs = es1 ++ es2 ->
+  fmap f (take (length es1) vs) = es1 /\ fmap f (drop (length es1) vs) = es2.
+Proof.
+  move => X Y f vs es1.
+  move : f vs.
+  elim: es1; destruct vs => //=.
+  move => es2 Hmap.
+  inversion Hmap; subst; clear Hmap.
+  apply H in H2. destruct H2; subst.
+  split => //=.
+  by f_equal.
+Qed.
+  
+Lemma fmap_insert_set_nth: forall T (l: list T) i vd v,
+  i < length l ->
+  <[i := v]> l = set_nth vd l i v.
+Proof.
+  move => T l i vd v Hlen.
+  move: i vd v Hlen.
+  induction l; move => i vd v Hlen; destruct i => //=; simpl in Hlen; try by lia.
+  apply lt_S_n in Hlen.
+  f_equal.
+  by apply IHl.
+Qed.
+
+Lemma list_fmap_app a b c d e :
+  list_fmap a b c (d ++ e) = list_fmap a b c d ++ list_fmap a b c e.
+Proof.
+  fold (fmap c (d ++ e)).
+  rewrite fmap_app.
+  done.
+Qed.
+
+Lemma those_projection_backward {T: Type} (l0: list (option T)) (l1: list T):
+  (forall k, match l0 !! k with
+        | Some x => x
+        | None => None
+        end
+        = l1 !! k) ->
+  length l0 = length l1 ->
+  those l0 = Some l1.
+Proof.
+  move: l0 l1.
+  induction l0; destruct l1 => //=; move => H Hlen.
+  specialize (H 0) as H0.
+  simpl in H0.
+  subst.
+  inversion Hlen; clear Hlen.
+  rewrite - those_those0.
+  simpl.
+  unfold option_map.
+  apply IHl0 in H1 => //; first by rewrite those_those0 H1.
+  move => k.
+  specialize (H (S k)).
+  by simpl in H.
+Qed.
+
+Lemma repeat_lookup {T: Type} (x: T) (n i: nat):
+  i < n <->
+  (repeat x n) !! i = Some x.
+Proof.
+  split. 
+  - move : n.
+    induction i; move => n HLen; destruct n => //=; try lia.
+    apply IHi.
+    lia.
+  - move => Hlookup.
+    apply lookup_lt_Some in Hlookup.
+    by rewrite repeat_length in Hlookup.
+Qed.
+
+Lemma repeat_lookup_None {T: Type} (x: T) (n i: nat):
+  i >= n <->
+  (repeat x n) !! i = None.
+Proof.
+  split. 
+  - move : n.
+    induction i; move => n HLen; destruct n => //=; try lia.
+    apply IHi.
+    lia.
+  - move => Hlookup.
+    apply lookup_ge_None in Hlookup.
+    by rewrite repeat_length in Hlookup.
+Qed.
+
+Lemma fmap_fmap_lookup {T1 T2 T: Type} (f1: T1 -> T) (f2: T2 -> T) (l1: list T1) (l2: list T2):
+  fmap f1 l1 = fmap f2 l2 ->
+  forall i, fmap f1 (l1 !! i) = fmap f2 (l2 !! i).
+Proof.
+  move => Heq i.
+  assert (length l1 = length l2) as Hlen.
+  { erewrite <- fmap_length with (f := f1).
+    rewrite Heq.
+    by rewrite fmap_length.
+  }
+  destruct (l1 !! i) eqn:Hl1; destruct (l2 !! i) eqn:Hl2 => //=.
+  - assert ((fmap f1 l1) !! i = (fmap f2 l2) !! i) as Heqi; first by rewrite Heq.
+    repeat rewrite list_lookup_fmap in Heqi.
+    rewrite Hl1 Hl2 in Heqi.
+    by simpl in Heqi.
+  - by apply lookup_lt_Some in Hl1; apply lookup_ge_None in Hl2; lias.
+  - by apply lookup_lt_Some in Hl2; apply lookup_ge_None in Hl1; lias.
+Qed.
